Helper functions

src/Iris/Algebra/Heap.lean
@@ -9,11 +9,10 @@ import Iris.Algebra.OFE
 
 open Iris
 
-/- # Datatype and CMRA for a generic heap-like structure.
-
-Like FunLike in Mathlib, but not exactly the same, since the type must also be able to be updated. -/
+/- # Datatype and CMRA for a generic heap-like structure. -/
 
 open Classical in
+/-- Update a (classical) function at a point. Used to specify the correctness of stores. -/
 noncomputable def fset {K V : Type _} (f : K → V) (k : K) (v : V) : K → V :=
   fun k' => if (k = k') then v else f k'
 
@@ -30,12 +29,27 @@ class Store (T : Type _) (K V : outParam (Type _)) extends StoreLike T K V where
   /-- One-sided inverse between get and of_fun. The other direction does not need to hold. -/
   of_fun_get {f} : get (of_fun f) = f
 
+class StoreIso (T : Type _) (K V : outParam (Type _)) extends Store T K V where
+  get_of_fun t : of_fun (get t) = t
+
+def StoreLike.map [StoreLike T1 K V1] [StoreLike T2 K V2] (t : T1) (f : V1 → V2) : T2 :=
+  StoreLike.of_fun <| f ∘ StoreLike.get t
+
+def StoreLike.merge [StoreLike T K V] (op : V → V → V) (t1 t2 : T) : T :=
+  StoreLike.of_fun <| (fun k => op (StoreLike.get t1 k) (StoreLike.get t2 k))
+
 class Alloc (T : Type _) (K : outParam (Type _)) where
   fresh : T → K
 
+class HeapLike (T : Type _) (K V : outParam (Type _)) extends StoreLike T K (Option V)
+
 /-- A type is HeapLike when it behaves like store for Optional values -/
-class Heap (T : Type _) (K V : outParam (Type _)) extends StoreLike T K (Option V), Alloc T K where
+class Heap (T : Type _) (K V : outParam (Type _)) extends HeapLike T K V, Alloc T K where
   fresh_get {t} : get t (fresh t) = none
+
+abbrev delete [HeapLike T K V] (t : T) (k : K) : T := StoreLike.set t k .none
+abbrev empty [HeapLike T K V] : T := StoreLike.of_fun (fun _ => .none)
+abbrev dom [HeapLike T K V] : T → K → Prop := fun t k => (StoreLike.get t k).isSome
 
 
 namespace Store
@@ -47,36 +61,99 @@ theorem get_set_ne {m : T} (H : k ≠ k') : get (set m k v) k' = get m k' := by
 theorem get_set_eq {m : T} (H : k = k') : get (set m k v) k' = v := by
   rw [get_set]; unfold fset; rw [if_pos H]
 
+theorem get_merge {op : V → V → V} (t1 t2 : T) (k : K) :
+    StoreLike.get (StoreLike.merge op t1 t2) k = op (StoreLike.get t1 k) (StoreLike.get t2 k) := by
+  unfold StoreLike.merge; rw [Store.of_fun_get]
+
 end Store
 
+theorem Store.get_map [StoreLike T1 K V1] [Store T2 K V2] {t : T1} {f : V1 → V2} {k : K} :
+    StoreLike.get (StoreLike.map t f : T2) k = f (StoreLike.get t k) := by
+  unfold StoreLike.map; rw [Store.of_fun_get]; rfl
 
 /-- Wrapper type for functions with the Store OFE -/
-structure StoreO (T : Type _) where car : T
+@[ext] structure StoreO (T : Type _) where car : T
 
-section algebra
+section ofe
 
-open OFE
+open OFE 
 
-/-- The OFE on StoreO is the discrete function OFE on it's .get function. -/
-instance StoreO_OFE {T K V : Type _} [StoreLike T K V] [OFE V] : OFE (StoreO T) where
+/-- The OFE on StoreO is the discrete function OFE on its .get function. -/
+instance StoreO_OFE [StoreLike T K V] [OFE V] : OFE (StoreO T) where
   Equiv s0 s1  := StoreLike.get s0.1 ≡ StoreLike.get s1.1
   Dist n s0 s1 := StoreLike.get s0.1 ≡{n}≡ StoreLike.get s1.1
   dist_eqv     := ⟨fun _ => .of_eq rfl, (·.symm), (·.trans ·)⟩
   equiv_dist   := equiv_dist
   dist_lt      := dist_lt
 
-def StoreO.toMap {T K V : Type _} [StoreLike T K V] [OFE V] : (StoreO T) -n> (K → V) where
+@[simp] def StoreO.toMap [StoreLike T K V] [OFE V] : (StoreO T) -n> (K → V) where
   f x := StoreLike.get <| StoreO.car x
   ne.1 {_ _ _} H k := H k
 
-def StoreO.ofMap {T K V : Type _} [Store T K V] [OFE V] : (K → V) -n> (StoreO T) where
+@[simp] def StoreO.ofMap [Store T K V] [OFE V] : (K → V) -n> (StoreO T) where
   f x := StoreO.mk <| StoreLike.of_fun x
   ne.1 {_ _ _} H k := by rw [Store.of_fun_get, Store.of_fun_get]; exact H k
 
-instance StoreO_COFE {T K V : Type _} [Store T K V] [COFE V] : COFE (StoreO T) where
+@[simp] def StoreO.get [StoreLike T K V] (k : K) : StoreO T → V :=
+  fun s => StoreLike.get s.1 k
+
+-- TODO: A `Proper` class could avoid the variable reordering.
+instance [StoreLike T K V] [OFE V] (k : K) : NonExpansive (StoreO.get k : StoreO T → V) where
+  ne {_ _ _} Ht := Ht k
+
+@[simp] def StoreO.set [StoreLike T K V] [OFE V] (k : K) : V → StoreO T → StoreO T :=
+  fun v s => StoreO.mk (StoreLike.set s.1 k v)
+
+-- TODO: A `Proper` class could avoid the variable reordering.
+instance [Store T K V] [OFE V] (k : K) : NonExpansive₂ (StoreO.set k : V → StoreO T → StoreO T) where
+  ne {n v1 v2} Hv {t1 t2} Ht k' := by
+    simp only [StoreO.set, Store.get_set, fset]
+    split
+    · exact Hv
+    · exact Ht k'
+
+@[simp] def StoreO.merge [StoreLike T K V] (op : V → V → V) (s1 s2 : StoreO T) : StoreO T :=
+  .mk (StoreLike.merge op s1.1 s2.1)
+
+instance [Store T K V] [OFE V] (op : V → V → V) [NonExpansive₂ op] :
+    NonExpansive₂ (StoreO.merge (T := T) op) where
+  ne n {_ _} Ht {_ _} Hs k := by
+    simp only [StoreO.merge, Store.get_merge]
+    exact NonExpansive₂.ne (Ht k) (Hs k)
+
+instance StoreO_COFE [Store T K V] [COFE V] : COFE (StoreO T) where
   compl c := ⟨StoreLike.of_fun <| COFE.compl <| c.map StoreO.toMap⟩
   conv_compl {n c} k := by
     rw [Store.of_fun_get]
     exact COFE.conv_compl (c := Chain.map StoreO.toMap c) k
 
-end algebra
+instance [Store T K V] [COFE V] [Discrete V] : Discrete (StoreO T) where
+  discrete_0 H k := discrete_0 <| H k
+
+/-- We can lift a Leibniz OFE on V to a Leibniz OFE on (StoreO T) as long as
+stores uniquely represent functions. -/
+instance [StoreIso T K V] [COFE V] [Leibniz V] : Leibniz (StoreO T) where
+  eq_of_eqv {x y} H := by
+    apply StoreO.ext
+    rewrite [← StoreIso.get_of_fun x.car, ← StoreIso.get_of_fun y.car]
+    congr 1
+    apply funext
+    intro k
+    apply eq_of_eqv (H k)
+
+end ofe
+
+
+section cmra
+
+/- ## A CMRA on Heaps
+TODO: I think there may be a generic way to put a CMRA on Stores, but I'm not sure of it. -/
+
+
+
+
+open CMRA
+
+
+
+end cmra
